formal/EvalFnTests.v
@@ -1,7 +1,8 @@
 (** I check reference-evaluator regressions by reduction in Rocq. These examples
     complement, rather than replace, the general soundness obligation. *)
-From Stdlib Require Import String ZArith Bool.
+From Stdlib Require Import String ZArith Bool List.
 From NanoCore Require Import Syntax EvalFn.
+Import ListNotations.
 Open Scope string_scope.
 Open Scope Z_scope.
 
@@ -55,3 +56,46 @@ Example logical_rejects_needed_nonbooleans :
   eval_fn 3 ENil (EBinOp OpAnd (EInt 0) (EBool false)) = None /\
   eval_fn 3 ENil (EBinOp OpOr (EInt 0) (EBool true)) = None.
 Proof. repeat split; reflexivity. Qed.
+
+Example arithmetic_zero_divisors_fail :
+  eval_fn 3 ENil (EBinOp OpDiv (EInt 7) (EInt 0)) = None /\
+  eval_fn 3 ENil (EBinOp OpMod (EInt 7) (EInt 0)) = None.
+Proof. split; reflexivity. Qed.
+
+Example let_restores_shadowed_binding :
+  eval_fn 6 logical_test_env
+    (ELet "x" (EInt 2) (ESeq (ESet "x" (EInt 3)) (EVar "x"))) =
+    Some (logical_test_env, VInt 3).
+Proof. reflexivity. Qed.
+
+Example let_preserves_outer_mutation :
+  eval_fn 6 logical_test_env (ELet "y" (EInt 2) (ESet "x" (EVar "y"))) =
+    Some (ECons "x" (VInt 2) ENil, VUnit).
+Proof. reflexivity. Qed.
+
+Example closure_body_does_not_mutate_caller :
+  eval_fn 6 logical_test_env
+    (EApp (ELam "y" TInt (ESeq (ESet "x" (EInt 9)) (EVar "y"))) (EInt 5)) =
+    Some (logical_test_env, VInt 5).
+Proof. reflexivity. Qed.
+
+Example recursive_closure_countdown :
+  eval_fn 12 ENil
+    (EApp (EFix "f" "n" TInt TInt
+      (EIf (EBinOp OpEq (EVar "n") (EInt 0)) (EInt 0)
+        (EApp (EVar "f") (EBinOp OpSub (EVar "n") (EInt 1))))) (EInt 2)) =
+    Some (ENil, VInt 0).
+Proof. reflexivity. Qed.
+
+Example while_threads_mutation :
+  eval_fn 10 logical_test_env
+    (EWhile (EBinOp OpLt (EVar "x") (EInt 2))
+      (ESet "x" (EBinOp OpAdd (EVar "x") (EInt 1)))) =
+    Some (ECons "x" (VInt 2) ENil, VUnit).
+Proof. reflexivity. Qed.
+
+Example match_restores_shadowed_binding :
+  eval_fn 5 logical_test_env
+    (EMatch (EConstruct "Some" (EInt 3) (TVariant [("Some", TInt)]))
+      [("Some", "x", EVar "x")]) = Some (logical_test_env, VInt 3).
+Proof. reflexivity. Qed.
